TransformerSemantics.v
@@ -1,3 +1,4 @@
+From Coq Require Import Program.Program.
 From VSA Require Import Basics.
 From VSA Require Import Functions.
 From VSA Require Import Lattice.
@@ -9,20 +10,21 @@ Import SetNotations.
 Variable P Q: Type.
 Context `{Setoid P} `{Setoid Q}.
 
-(* TODO: solve type_classes priorities *)
-Set Printing Implicit.
-
 #[program]
 Definition post (R: ℘ (P * Q)): { f : (℘ P -> ℘ Q) | PreserveSup f } :=
   fun p y => exists x, x ∈ p /\ R (x, y).
 Next Obligation.
-  intros S y.
+  intros S y. split.
+  - intros [x [[T [H__T H__x]] H__R]]. exists (fun y' => exists x', T x' /\ R (x', y')). firstorder.
+  - intros [T1 [[T [H__T H__T1]] H__y]]; subst. firstorder.
+Qed.
 
 Definition post_inv (T: { f : (℘ P -> ℘ Q) | PreserveSup f }): ℘ (P * Q) :=
-  fun xy => (snd xy) ∈ T {{ (fst xy) }}.
+  fun xy => (snd xy) ∈ `T {{ (fst xy) }}.
 
+(*
 Definition post_dual (R: ℘ (P * Q)): ℘ P -> ℘ Q :=
-  fun p => ¬ (post R (¬ p)).
+  fun p => ¬ (post R (¬ p)). *)
 
 Print GaloisConnection.
 
@@ -31,14 +33,18 @@ Instance post_post_inv_connection:
   GaloisConnection (℘ (P * Q)) ({ f : (℘ P -> ℘ Q) | PreserveSup f }) post post_inv.
 Next Obligation.
   split; intros H.
-  - intros xy H__xy.
-    apply H. exists (fst xy).
-    split.
-    + reflexivity.
-    + rewrite <- surjective_pairing with P Q xy. assumption.
+  - intros xy H__xy. apply H. exists (fst xy). split.
+     reflexivity.
+    rewrite <- surjective_pairing with P Q xy. assumption.
   - intros p y [x [H__x H__R]].
     unfold gamma in H. unfold post_inv in H.
     unfold ord in H. unfold PowersetOrd in H.
+    assert (Q0 {{ x }} ⊆ Q0 p).
+    {
+      intros y' H'.
+    }
+    simpl.
+    (* Decomposition of a set into each element??? *)
     (* Use the fact that it is U-morphism *)
     apply H.
 
